an equivalent form of unification

doc/simple/coq/UtilityAlgo.v
@@ -1614,3 +1614,1232 @@ Theorem unify_extension: forall G s t H,
     AWf G ->
     AWf H /\ ExtCtx G H.
 Admitted.
+
+(***********************)
+(* EQUIVALENCE OF UNIFY *)
+(***********************)
+
+Inductive AUMode := UType | UExpr.
+
+Inductive ATUnify : AUMode -> ACtx -> AType -> AType -> ACtx -> Prop :=
+  | ATUnify_Var : forall x G, binds x AC_Var G -> ATUnify UExpr G (AT_Expr (AE_FVar x)) (AT_Expr (AE_FVar x)) G
+  | ATUnify_Typed_Var : forall x G t, binds x (AC_Typ t) G -> ATUnify UExpr G (AT_Expr (AE_FVar x)) (AT_Expr (AE_FVar x)) G
+  | ATUnify_EVar : forall a G, binds a AC_Unsolved_EVar G -> ATUnify UType G (AT_EVar a) (AT_EVar a) G
+  | ATUnify_TVar : forall a G, binds a AC_TVar G -> ATUnify UType G (AT_TFVar a) (AT_TFVar a) G
+  | ATUnify_Star : forall G, ATUnify UExpr G (AT_Expr (AE_Star)) (AT_Expr (AE_Star)) G
+  | ATUnify_App : forall t1 t2 t3 t4 G H1 H,
+      ATUnify UExpr G (AT_Expr t1) (AT_Expr t2) H1 ->
+      ATUnify UExpr H1 (AT_Expr (ACtxSubst H1 t3)) (AT_Expr (ACtxSubst H1 t4)) H ->
+      ATUnify UExpr G (AT_Expr (AE_App t1 t3)) (AT_Expr (AE_App t2 t4)) H
+  | ATUnify_Lam : forall t1 t2 G H L,
+      (forall x, x \notin L -> ATUnify UExpr (G & x ~ AC_Var) (AT_Expr (t1 @ x)) (AT_Expr (t2 @ x)) (H & x ~ AC_Var)) ->
+      ATUnify UExpr G (AT_Expr (AE_Lam t1)) (AT_Expr (AE_Lam t2)) H
+  | ATUnify_CastUp : forall t1 t2 G H,
+      ATUnify UExpr G (AT_Expr t1) (AT_Expr t2) H ->
+      ATUnify UExpr G (AT_Expr (AE_CastUp t1)) (AT_Expr (AE_CastUp t2)) H
+  | ATUnify_CastDn : forall t1 t2 G H,
+      ATUnify UExpr G (AT_Expr t1) (AT_Expr t2) H ->
+      ATUnify UExpr G (AT_Expr (AE_CastDn t1)) (AT_Expr (AE_CastDn t2)) H
+  | ATUnify_Pi : forall t1 t2 t3 t4 G H1 H L,
+      ATUnify UType G t1 t3 H1 ->
+      (forall x, x \notin L -> ATUnify UType (H1 & x ~ AC_Typ t1) (ACtxTSubst H1 (t2 @' x)) (ACtxTSubst H1 (t4 @' x)) (H & x ~ AC_Typ t1)) ->
+      ATUnify UExpr G (AT_Expr (AE_Pi t1 t2)) (AT_Expr (AE_Pi t3 t4)) H
+  | ATUnify_Forall : forall t1 t2 G H L,
+      (forall x, x \notin L -> ATUnify UType (G & x ~ AC_TVar) (t1 @#' x) (t2 @#' x) (H & x ~ AC_TVar)) ->
+      ATUnify UExpr G (AT_Expr (AE_Forall t1)) (AT_Expr (AE_Forall t2)) H
+  | ATUnify_Ann : forall t1 t2 t3 t4 G H1 H,
+      ATUnify UExpr G (AT_Expr t1) (AT_Expr t2) H1 ->
+      ATUnify UType H1 (ACtxTSubst H1 t3) (ACtxTSubst H1 t4) H ->
+      ATUnify UExpr G (AT_Expr (AE_Ann t1 t3)) (AT_Expr (AE_Ann t2 t4)) H
+  | ATUnify_EVarTy : forall a t1 t2 G H1 H2,
+      a \notin ATFv (t1) ->
+      AResolveEVar G a t1 t2 (H1 & a ~ AC_Unsolved_EVar & H2) ->
+      AWTermT H1 t2 ->
+      ATUnify UType G (AT_EVar a) t1 (H1 & a ~ AC_Solved_EVar t2 & H2)
+  | ATUnify_TyEVar : forall a t1 t2 G H1 H2,
+      (forall n, t1 <> AT_EVar n) ->
+      a \notin ATFv (t1) ->
+      AResolveEVar G a t1 t2 (H1 & a ~ AC_Unsolved_EVar & H2) ->
+      AWTermT H1 t2 ->
+      ATUnify UType G t1 (AT_EVar a) (H1 & a ~ AC_Solved_EVar t2 & H2)
+  | ATUnify_Expr: forall G t1 t2 H,
+      ATUnify UExpr G t1 t2 H ->
+      ATUnify UType G t1 t2 H.
+
+Lemma atunify_ok_preservation: forall G m s t H,
+    ATUnify m G s t H ->
+    ok G ->
+    ok H.
+Proof.
+  introv uni okg.
+  induction uni; auto.
+
+  pick_fresh y.
+  assert (y \notin L) by auto_star.
+  assert (ok (G & y ~ AC_Var)) by apply* ok_push.
+  lets: H1 H2 H3.
+  apply ok_concat_inv_l in H4; auto.
+
+  pick_fresh y.
+  assert (y \notin L) by auto_star.
+  lets: H2 H3. clear H2.
+  assert (ok (H1 & y ~ AC_Typ t1)) by apply* ok_push.
+  lets: H4 H2.
+  apply ok_concat_inv_l in H5; auto.
+
+  pick_fresh y.
+  assert (y \notin L) by auto_star.
+  assert (ok (G & y ~ AC_TVar)) by apply* ok_push.
+  lets: H1 H2 H3.
+  apply ok_concat_inv_l in H4; auto.
+
+  lets: resolve_evar_ok_preservation H0 okg.
+  apply* ok_middle_change.
+
+  lets: resolve_evar_ok_preservation H3 okg.
+  apply* ok_middle_change.
+Qed.
+
+Lemma resolve_evar_middle_change: forall G1 G2 a t H1 H2 t2 v a0,
+    AResolveEVar (G1 & a ~ AC_Typ t & G2) a0 v t2
+                 (H1 & a ~ AC_Typ t & H2) ->
+    ok (G1 & a ~ AC_Typ t & G2) ->
+    AResolveEVar (G1 & a ~ AC_Var & G2) a0 v t2
+                 (H1 & a ~ AC_Var & H2).
+Proof.
+  introv res okg.
+  gen_eq S1: (G1 & a ~ AC_Typ t & G2).
+  gen_eq S2: (H1 & a ~ AC_Typ t & H2). gen H1 H2 G1 G2.
+  lets: resolve_evar_ok_preservation res okg.
+  induction res; introv sinfo1 sinfo2; subst; auto;
+    try(solve[apply ok_middle_eq2 in sinfo2; auto;
+              try(destruct sinfo2 as [? [_ ?]]; subst; constructor~);
+              try(rewrite~ <- sinfo2)]).
+
+  (* EVAR BEFORE *)
+  assert (binds a (AC_Typ t) (H1 & a ~ AC_Typ t & H2)).
+  apply binds_middle_eq. rewrite sinfo1 in okg. apply ok_middle_inv_r in okg. auto.
+  assert (a <> b). introv neq. subst.
+  rewrite <- sinfo1 in H0. do 2 rewrite <- concat_assoc in H0.
+  false binds_middle_eq_inv H0.
+  repeat rewrite~ concat_assoc.
+  assert (a <> a0). introv neq. subst.
+  rewrite <- sinfo1 in H0.
+  false binds_middle_eq_inv H0; auto.
+
+  rewrite <- sinfo1 in H0.
+  apply binds_remove in H0; auto.
+  rewrite <- concat_assoc in H0.
+  apply binds_remove in H0; auto.
+  rewrite concat_assoc in H0.
+  apply binds_concat_inv in H0.
+  destruct H0 as [bdg3 | [noting3 bdg1g2]].
+  apply split_bind_context in bdg3.
+  destruct bdg3 as (I1 & I2 & g3info). subst.
+  repeat rewrite concat_assoc in sinfo2.
+  apply ok_middle_eq2 in sinfo2; auto.
+  destruct sinfo2 as [? [_ ?]]. subst.
+  repeat rewrite concat_assoc in sinfo1.
+  apply ok_middle_eq2 in sinfo1; auto.
+  destruct sinfo1 as [? [_ ?]]. subst.
+
+  assert(
+      AResolveEVar
+     (G1 & b ~ AC_Unsolved_EVar & G2 & a0 ~ AC_Unsolved_EVar & (I1 & a ~ AC_Var & H2))
+     a0 (AT_EVar b) (AT_EVar b)
+     (G1 & b ~ AC_Unsolved_EVar & G2 & a0 ~ AC_Unsolved_EVar & (I1 & a ~ AC_Var & H2))).
+  apply~ AResolveEVar_EVar_Before.
+  repeat rewrite concat_assoc in H0; auto.
+
+  repeat rewrite concat_assoc in H. auto.
+  rewrite <- sinfo1.
+  repeat rewrite concat_assoc in H. auto.
+  repeat rewrite concat_assoc in H. auto.
+  rewrite <- sinfo2.
+  repeat rewrite concat_assoc in H. auto.
+
+  apply binds_concat_inv in bdg1g2.
+  destruct bdg1g2 as [bdg2 | [noting2 bdg1]].
+  apply split_bind_context in bdg2.
+  destruct bdg2 as (I1 & I2 & g2info). subst.
+  repeat rewrite concat_assoc in sinfo2.
+  do 2 rewrite <- concat_assoc in sinfo2.
+  apply ok_middle_eq2 in sinfo2; auto.
+  destruct sinfo2 as [? [_ ?]]. subst.
+  repeat rewrite concat_assoc in sinfo1.
+  do 2 rewrite <- concat_assoc in sinfo1.
+  apply ok_middle_eq2 in sinfo1; auto.
+  destruct sinfo1 as [? [_ ?]]. subst.
+
+  assert(
+   AResolveEVar
+     (G1 & b ~ AC_Unsolved_EVar & (I1 & a ~ AC_Var & I2) & a0 ~ AC_Unsolved_EVar & G3)
+     a0 (AT_EVar b) (AT_EVar b)
+     (G1 & b ~ AC_Unsolved_EVar & (I1 & a ~ AC_Var & I2) & a0 ~ AC_Unsolved_EVar & G3)).
+  apply~ AResolveEVar_EVar_Before.
+  repeat rewrite concat_assoc in H0; auto.
+  repeat rewrite concat_assoc. auto.
+
+  repeat rewrite concat_assoc in *. auto.
+  rewrite <- sinfo1.
+  repeat rewrite concat_assoc in *. auto.
+  repeat rewrite concat_assoc in *. auto.
+  rewrite <- sinfo2.
+  repeat rewrite concat_assoc in *. auto.
+
+  apply split_bind_context in bdg1.
+  destruct bdg1 as (I1 & I2 & g2info). subst.
+  do 4 rewrite <- concat_assoc in sinfo2.
+  apply ok_middle_eq2 in sinfo2; auto.
+  destruct sinfo2 as [? [_ ?]]. subst.
+  do 4 rewrite <- concat_assoc in sinfo1.
+  apply ok_middle_eq2 in sinfo1; auto.
+  destruct sinfo1 as [? [_ ?]]. subst.
+
+  repeat rewrite concat_assoc in *.
+  apply~ AResolveEVar_EVar_Before.
+
+  repeat rewrite concat_assoc in *. auto.
+  rewrite <- sinfo1.
+  repeat rewrite concat_assoc in *. auto.
+  repeat rewrite concat_assoc in *. auto.
+  rewrite <- sinfo2.
+  repeat rewrite concat_assoc in *. auto.
+
+  (* EVAR AFTER *)
+  assert( ok (H1 & a ~ AC_Typ t & H2)). rewrite <- sinfo1.
+  do 3 rewrite <- concat_assoc.
+  apply ok_insert; auto.
+  repeat rewrite concat_assoc.
+  apply* ok_middle_change.
+
+  assert (binds a (AC_Typ t) (H1 & a ~ AC_Typ t & H2)).
+  apply binds_middle_eq. apply ok_middle_inv_r in H3. auto.
+  assert (a <> b). introv neq. subst.
+  rewrite <- sinfo1 in H4.
+  false binds_middle_eq_inv H4.
+  rewrite~ sinfo1.
+  assert (a <> a0). introv neq. subst.
+  rewrite <- sinfo1 in H4.
+  do 2 rewrite <- concat_assoc in H4.
+  false binds_middle_eq_inv H4; auto.
+  repeat rewrite~ concat_assoc.
+  assert (a <> a1). introv neq. subst.
+  rewrite <- sinfo1 in H4.
+  do 3 rewrite <- concat_assoc in H4.
+  false binds_middle_eq_inv H4; auto.
+  repeat rewrite~ concat_assoc.
+
+  rewrite <- sinfo1 in H4.
+  apply binds_remove in H4; auto.
+  rewrite <- concat_assoc in H4.
+  apply binds_remove in H4; auto.
+  apply binds_remove in H4; auto.
+  rewrite concat_assoc in H4.
+  apply binds_concat_inv in H4.
+  destruct H4 as [bdg3 | [noting3 bdg1g2]].
+  apply split_bind_context in bdg3.
+  destruct bdg3 as (I1 & I2 & g3info). subst.
+  repeat rewrite concat_assoc in sinfo2.
+  apply ok_middle_eq2 in sinfo2; auto.
+  destruct sinfo2 as [? [_ ?]]. subst.
+  repeat rewrite concat_assoc in sinfo1.
+  apply ok_middle_eq2 in sinfo1; auto.
+  destruct sinfo1 as [? [_ ?]]. subst.
+
+  assert(
+   AResolveEVar
+     (G1 & a0 ~ AC_Unsolved_EVar & G2 & b ~ AC_Unsolved_EVar & (I1 & a ~ AC_Var & H2))
+     a0 (AT_EVar b) (AT_EVar a1)
+     (G1 & a1 ~ AC_Unsolved_EVar & a0 ~ AC_Unsolved_EVar & G2 & b ~ AC_Solved_EVar (AT_EVar a1) & (I1 & a ~ AC_Var & H2))).
+  apply~ AResolveEVar_EVar_After.
+  repeat rewrite concat_assoc in H1; auto.
+
+  repeat rewrite concat_assoc in *. auto.
+  repeat rewrite concat_assoc in *. auto.
+  rewrite <- sinfo2.
+  repeat rewrite concat_assoc in *. auto.
+
+  apply binds_concat_inv in bdg1g2.
+  destruct bdg1g2 as [bdg2 | [noting2 bdg1]].
+  apply split_bind_context in bdg2.
+  destruct bdg2 as (I1 & I2 & g2info). subst.
+  repeat rewrite concat_assoc in sinfo2.
+  do 2 rewrite <- concat_assoc in sinfo2.
+  apply ok_middle_eq2 in sinfo2; auto.
+  destruct sinfo2 as [? [_ ?]]. subst.
+  repeat rewrite concat_assoc in sinfo1.
+  do 2 rewrite <- concat_assoc in sinfo1.
+  apply ok_middle_eq2 in sinfo1; auto.
+  destruct sinfo1 as [? [_ ?]]. subst.
+
+  repeat rewrite concat_assoc.
+  assert(
+   AResolveEVar
+     (G1 & a0 ~ AC_Unsolved_EVar & (I1 & a ~ AC_Var & I2) &
+      b ~ AC_Unsolved_EVar & G3) a0 (AT_EVar b) (AT_EVar a1)
+     (G1 & a1 ~ AC_Unsolved_EVar & a0 ~ AC_Unsolved_EVar & (I1 & a ~ AC_Var &
+      I2) & b ~ AC_Solved_EVar (AT_EVar a1) & G3)).
+  apply~ AResolveEVar_EVar_After.
+  repeat rewrite concat_assoc in *; auto.
+
+  repeat rewrite concat_assoc in *. auto.
+  repeat rewrite concat_assoc in *. auto.
+  rewrite <- sinfo2.
+  repeat rewrite concat_assoc in *. auto.
+
+  apply split_bind_context in bdg1.
+  destruct bdg1 as (I1 & I2 & g2info). subst.
+  do 4 rewrite <- concat_assoc in sinfo2.
+  apply ok_middle_eq2 in sinfo2; auto.
+  destruct sinfo2 as [? [_ ?]]. subst.
+  do 5 rewrite <- concat_assoc in sinfo1.
+  apply ok_middle_eq2 in sinfo1; auto.
+  destruct sinfo1 as [? [_ ?]]. subst.
+
+  repeat rewrite concat_assoc.
+  apply~ AResolveEVar_EVar_After.
+  repeat rewrite concat_assoc in *; auto.
+
+  repeat rewrite concat_assoc in *. auto.
+  rewrite <- sinfo2.
+  repeat rewrite concat_assoc in *. auto.
+
+
+  (* PI *)
+  lets: resolve_evar_wextctx res okg.
+  apply weak_extension_order_typvar in H0.
+  destruct H0 as (I1 & I2 & [hinfo _]).
+  subst.
+  lets: resolve_evar_ok_preservation res okg.
+  apply AResolveEVar_Pi with (L:=L \u dom (I1 & a ~ AC_Typ t & I2) \u dom (H4 & a ~ AC_Typ t & H5)) (H1:=(I1 & a ~ AC_Var & I2)).
+  forwards * : IHres. clear IHres.
+  intros y notin.
+  assert(y \notin L) by auto.
+  lets: H2 H1. clear H2.
+  assert(H4 & a ~ AC_Typ t & H5 & y ~ AC_Var = H4 & a ~ AC_Typ t & (H5 & y ~ AC_Var )) by repeat rewrite~ concat_assoc.
+  assert(I1 & a ~ AC_Typ t & I2 & y ~ AC_Var = I1 & a ~ AC_Typ t & (I2 & y ~ AC_Var)) by  repeat rewrite~ concat_assoc.
+  assert (ok (I1 & a ~ AC_Typ t & I2 & y ~ AC_Var)) by apply~ ok_push.
+  lets: H3 H1 H8 H2 H7. apply~ ok_push.
+  repeat rewrite concat_assoc in H9; auto.
+
+  rewrite tsubst_add_ctx in H9. rewrite tsubst_add_typvar in H9.
+  rewrite tsubst_add_ctx. rewrite tsubst_add_var. auto.
+
+  (* APP *)
+  lets: resolve_evar_wextctx res1 okg.
+  apply weak_extension_order_typvar in H0.
+  destruct H0 as (I1 & I2 & [hinfo _]). subst.
+  lets: resolve_evar_ok_preservation res1 okg.
+  lets: resolve_evar_ok_preservation res2 H0.
+  forwards * : IHres1. clear IHres1.
+  forwards * : IHres2. clear IHres2.
+  apply* AResolveEVar_App.
+
+  rewrite tsubst_add_ctx in H5. rewrite tsubst_add_typvar in H5.
+  rewrite tsubst_add_ctx. rewrite tsubst_add_var. auto.
+
+  (* LAM *)
+  apply AResolveEVar_Lam with (L \u dom (G1 & a ~ AC_Typ t & G2) \u dom (H3 & a ~ AC_Typ t & H4)).
+  intros y notin.
+  assert(y \notin L) by auto.
+  lets: H1 H0. clear H1.
+  assert(H3 & a ~ AC_Typ t & H4 & y ~ AC_Var = H3 & a ~ AC_Typ t & (H4 & y ~ AC_Var )) by repeat rewrite~ concat_assoc.
+  assert(G1 & a ~ AC_Typ t & G2 & y ~ AC_Var = G1 & a ~ AC_Typ t & (G2 & y ~ AC_Var)) by  repeat rewrite~ concat_assoc.
+  assert (ok (G1 & a ~ AC_Typ t & G2 & y ~ AC_Var)) by apply~ ok_push.
+  assert (ok (H3 & a ~ AC_Typ t & H4 & y ~ AC_Var)) by apply~ ok_push.
+  lets: H2 H0 H7 H8 H1 H6.
+  repeat rewrite concat_assoc in H9; auto.
+
+  (* ANN *)
+  lets: resolve_evar_wextctx res1 okg.
+  apply weak_extension_order_typvar in H0.
+  destruct H0 as (I1 & I2 & [hinfo _]). subst.
+  lets: resolve_evar_ok_preservation res1 okg.
+  lets: resolve_evar_ok_preservation res2 H0.
+  forwards * : IHres1. clear IHres1.
+  forwards * : IHres2. clear IHres2.
+  apply* AResolveEVar_Ann.
+
+  rewrite tsubst_add_ctx in H5. rewrite tsubst_add_typvar in H5.
+  rewrite tsubst_add_ctx. rewrite tsubst_add_var. auto.
+Qed.
+
+Lemma aunify_middle_change: forall e G1 G2 a t d H1 H2,
+    AUnify (G1 & a ~ AC_Typ t & G2) e d (H1 & a ~ AC_Typ t & H2) ->
+    ok (G1 & a ~ AC_Typ t & G2) ->
+    AUnify (G1 & a ~ AC_Var & G2) e d (H1 & a ~ AC_Var & H2).
+Proof.
+  introv uni.
+  gen_eq S1: (G1 & a ~ AC_Typ t & G2).
+  gen_eq S2: (H1 & a ~ AC_Typ t & H2). gen H1 H2 G1 G2.
+  induction uni; introv sinfo1 sinfo2 okg; subst.
+
+  (* Var *)
+  assert (x <> a). introv neq. subst. false binds_middle_eq_inv H. auto.
+  apply binds_remove in H; auto.
+  apply ok_middle_eq2 in sinfo2; auto.
+  destruct sinfo2 as [? [_ ?]]. subst.
+  apply AUnify_Var. apply~ binds_weaken.
+  apply* ok_middle_change.
+  rewrite <- sinfo2. auto.
+
+  (* TypedVar *)
+  apply ok_middle_eq2 in sinfo2; auto.
+  destruct sinfo2 as [? [_ ?]]. subst.
+  destruct(eq_var_dec x a).
+  subst.
+  apply~ AUnify_Var. apply~ binds_middle_eq.
+  apply ok_middle_inv_r in okg. auto.
+  apply AUnify_Typed_Var with t0.
+  apply binds_remove in H; auto.
+  apply~ binds_weaken.
+  apply* ok_middle_change.
+  rewrite <- sinfo2. auto.
+
+  (* EVar *)
+  assert (a0 <> a). introv neq. subst. false binds_middle_eq_inv H. auto.
+  apply binds_remove in H; auto.
+  apply ok_middle_eq2 in sinfo2; auto.
+  destruct sinfo2 as [? [_ ?]]. subst.
+  apply AUnify_EVar. apply~ binds_weaken.
+  apply* ok_middle_change.
+  rewrite <- sinfo2. auto.
+
+  (* TFVar *)
+  assert (a0 <> a). introv neq. subst. false binds_middle_eq_inv H. auto.
+  apply binds_remove in H; auto.
+  apply ok_middle_eq2 in sinfo2; auto.
+  destruct sinfo2 as [? [_ ?]]. subst.
+  apply AUnify_TVar. apply~ binds_weaken.
+  apply* ok_middle_change.
+  rewrite <- sinfo2. auto.
+
+  (* STAR *)
+  apply ok_middle_eq2 in sinfo2; auto.
+  destruct sinfo2 as [? [_ ?]]. subst.
+  apply AUnify_Star.
+  rewrite <- sinfo2. auto.
+
+  (* APP *)
+  lets: unify_wextctx uni1 okg.
+  apply weak_extension_order_typvar in H.
+  destruct H as (I1 & I2 & [hinfo _]). subst.
+  lets: unify_ok_preservation uni1 okg.
+  forwards * : IHuni1. clear IHuni1.
+  forwards * : IHuni2. clear IHuni2.
+  apply* AUnify_App.
+  rewrite subst_add_ctx in H3.
+  rewrite subst_add_typvar in H3.
+  rewrite subst_add_ctx in H3.
+  rewrite subst_add_typvar in H3.
+  rewrite subst_add_ctx.
+  rewrite subst_add_var.
+  rewrite subst_add_ctx.
+  rewrite subst_add_var. auto.
+
+  (* LAM *)
+  apply AUnify_Lam with (L \u dom (G1 & a ~ AC_Typ t & G2)).
+  intros y notin.
+  assert(H: y \notin L) by auto.
+  lets: H0 H. clear H0.
+  assert(H2 & a ~ AC_Typ t & H3 & y ~ AC_Var = H2 & a ~ AC_Typ t & (H3 & y ~ AC_Var )) by repeat rewrite~ concat_assoc.
+  assert(G1 & a ~ AC_Typ t & G2 & y ~ AC_Var = G1 & a ~ AC_Typ t & (G2 & y ~ AC_Var)) by  repeat rewrite~ concat_assoc.
+  assert (ok (G1 & a ~ AC_Typ t & G2 & y ~ AC_Var)) by apply~ ok_push.
+  lets: H1 H H0 H5 H6.
+  repeat rewrite concat_assoc in H7; auto.
+
+  (* CASTUP *)
+  forwards * : IHuni.
+
+  (* CASTDOWN *)
+  forwards * : IHuni.
+
+  (* PI *)
+  lets: unify_wextctx uni okg.
+  apply weak_extension_order_typvar in H.
+  destruct H as (I1 & I2 & [hinfo _]). subst.
+  lets: unify_ok_preservation uni okg.
+  apply AUnify_Pi with (L:=L \u dom (I1 & a ~ AC_Typ t & I2)) (H1:=(I1 & a ~ AC_Var & I2)).
+  forwards * : IHuni. clear IHuni.
+  intros y notin.
+  assert(y \notin L) by auto.
+  lets: H0 H1. clear H0.
+  assert(H3 & a ~ AC_Typ t & H4 & y ~ AC_Var = H3 & a ~ AC_Typ t & (H4 & y ~ AC_Var )) by repeat rewrite~ concat_assoc.
+  assert(I1 & a ~ AC_Typ t & I2 & y ~ AC_Var = I1 & a ~ AC_Typ t & (I2 & y ~ AC_Var)) by  repeat rewrite~ concat_assoc.
+  assert (ok (I1 & a ~ AC_Typ t & I2 & y ~ AC_Var)) by apply~ ok_push.
+  lets: H2 H1 H0 H6 H7.
+  repeat rewrite concat_assoc in H8; auto.
+
+  rewrite tsubst_add_ctx in H8. rewrite tsubst_add_typvar in H8.
+  rewrite tsubst_add_ctx in H8. rewrite tsubst_add_typvar in H8.
+  rewrite tsubst_add_ctx. rewrite tsubst_add_var.
+  rewrite tsubst_add_ctx. rewrite tsubst_add_var. auto.
+
+  (* FORALL *)
+  apply AUnify_Forall with (L \u dom (G1 & a ~ AC_Typ t & G2)).
+  intros y notin.
+  assert(H: y \notin L) by auto.
+  lets: H0 H. clear H0.
+  assert(H2 & a ~ AC_Typ t & H3 & y ~ AC_TVar = H2 & a ~ AC_Typ t & (H3 & y ~ AC_TVar )) by repeat rewrite~ concat_assoc.
+  assert(G1 & a ~ AC_Typ t & G2 & y ~ AC_TVar = G1 & a ~ AC_Typ t & (G2 & y ~ AC_TVar)) by  repeat rewrite~ concat_assoc.
+  assert (ok (G1 & a ~ AC_Typ t & G2 & y ~ AC_TVar)) by apply~ ok_push.
+  lets: H1 H H0 H5 H6.
+  repeat rewrite concat_assoc in H7; auto.
+
+  (* ANN *)
+  lets: unify_wextctx uni1 okg.
+  apply weak_extension_order_typvar in H.
+  destruct H as (I1 & I2 & [hinfo _]). subst.
+  lets: unify_ok_preservation uni1 okg.
+  forwards * : IHuni1. clear IHuni1.
+  forwards * : IHuni2. clear IHuni2.
+  apply* AUnify_Ann.
+  rewrite tsubst_add_ctx in H3. rewrite tsubst_add_typvar in H3.
+  rewrite tsubst_add_ctx in H3. rewrite tsubst_add_typvar in H3.
+  rewrite tsubst_add_ctx. rewrite tsubst_add_var.
+  rewrite tsubst_add_ctx. rewrite tsubst_add_var. auto.
+
+  (* EVAR TY *)
+  lets: resolve_evar_ok_preservation H0 okg.
+  assert(binds a0 (AC_Solved_EVar t2) (H1 & a0 ~ AC_Solved_EVar t2 & H2)).
+  apply~ binds_middle_eq. apply ok_middle_inv_r in H6; auto.
+  rewrite sinfo1 in H7.
+  apply binds_remove in H7; auto.
+  apply binds_concat_inv in H7.
+  destruct H7 as [bdh2 | [notinh2 bdh1]].
+  apply split_bind_context in bdh2.
+  destruct bdh2 as (I1 & I2 & g2info). subst.
+  repeat rewrite concat_assoc in *.
+  apply ok_middle_eq2 in sinfo1; auto.
+  destruct sinfo1 as [? [_ ?]]. subst.
+  apply~ AUnify_EVarTy.
+  do 3 rewrite <- concat_assoc in H0.
+  rewrite concat_assoc in H0.
+  apply resolve_evar_middle_change in H0; auto.
+  repeat rewrite concat_assoc in H0. auto.
+  apply* awtermt_replace.
+  apply* ok_middle_change.
+  rewrite <- sinfo1. apply* ok_middle_change.
+
+  apply split_bind_context in bdh1.
+  destruct bdh1 as (I1 & I2 & g2info). subst.
+  do 3 rewrite <- concat_assoc in sinfo1.
+  rewrite concat_assoc in sinfo1.
+  apply ok_middle_eq2 in sinfo1; auto.
+  destruct sinfo1 as [? [_ ?]]. subst.
+  do 3 rewrite <- concat_assoc.
+  rewrite concat_assoc.
+  apply~ AUnify_EVarTy.
+  repeat rewrite concat_assoc in H0.
+  apply resolve_evar_middle_change in H0; auto.
+  repeat rewrite concat_assoc. auto.
+  apply* ok_middle_change.
+  rewrite <- sinfo1. apply* ok_middle_change.
+
+  assert(a0 <> a). introv neq. subst. false binds_middle_eq_inv H7.
+  rewrite~ <- sinfo1. apply* ok_middle_change.
+  auto.
+
+  (* TY EVAR *)
+  lets: resolve_evar_ok_preservation H3 okg.
+  assert(binds a0 (AC_Solved_EVar t2) (H1 & a0 ~ AC_Solved_EVar t2 & H2)).
+  apply~ binds_middle_eq. apply ok_middle_inv_r in H7; auto.
+  rewrite sinfo1 in H8.
+  apply binds_remove in H8; auto.
+  apply binds_concat_inv in H8.
+  destruct H8 as [bdh2 | [notinh2 bdh1]].
+  apply split_bind_context in bdh2.
+  destruct bdh2 as (I1 & I2 & g2info). subst.
+  repeat rewrite concat_assoc in *.
+  apply ok_middle_eq2 in sinfo1; auto.
+  destruct sinfo1 as [? [_ ?]]. subst.
+  apply~ AUnify_TyEVar.
+  do 3 rewrite <- concat_assoc in H3.
+  rewrite concat_assoc in H3.
+  apply resolve_evar_middle_change in H3; auto.
+  repeat rewrite concat_assoc in H3. auto.
+  apply* awtermt_replace.
+  apply* ok_middle_change.
+  rewrite <- sinfo1. apply* ok_middle_change.
+
+  apply split_bind_context in bdh1.
+  destruct bdh1 as (I1 & I2 & g2info). subst.
+  do 3 rewrite <- concat_assoc in sinfo1.
+  rewrite concat_assoc in sinfo1.
+  apply ok_middle_eq2 in sinfo1; auto.
+  destruct sinfo1 as [? [_ ?]]. subst.
+  do 3 rewrite <- concat_assoc.
+  rewrite concat_assoc.
+  apply~ AUnify_TyEVar.
+  repeat rewrite concat_assoc in H3.
+  apply resolve_evar_middle_change in H3; auto.
+  repeat rewrite concat_assoc. auto.
+  apply* ok_middle_change.
+  rewrite <- sinfo1. apply* ok_middle_change.
+
+  assert(a0 <> a). introv neq. subst. false binds_middle_eq_inv H8.
+  rewrite~ <- sinfo1. apply* ok_middle_change.
+  auto.
+Qed.
+
+Lemma atunify_is_aunify: forall G m s t H,
+    ok G ->
+    ATUnify m G s t H ->
+    AUnify G s t H.
+Proof.
+  introv okg uni.
+  induction uni; auto.
+  apply AUnify_Typed_Var with t; auto.
+
+  lets: atunify_ok_preservation uni1 okg.
+  apply* AUnify_App.
+
+  apply AUnify_Lam with (L \u dom G).
+  intros y notin.
+  assert(y \notin L) by auto.
+  assert(ok (G & y ~ AC_Var)) by apply~ ok_push.
+  lets: H1 H2 H3. auto.
+
+  apply AUnify_Pi with (L:=L \u dom H1) (H1:=H1); auto.
+  intros y notin.
+  assert(y \notin L) by auto.
+  lets: H2 H3. clear H2.
+  lets: IHuni okg. clear IHuni.
+  lets: unify_ok_preservation H2 okg.
+  assert( ok (H1 & y ~ AC_Typ t1)) by apply~ ok_push.
+  lets: H4 H6. clear H4.
+  assert( AUnify (H1 & y ~ AC_Typ t1 & empty) (ACtxTSubst H1 (t2 @@' AE_FVar y))
+         (ACtxTSubst H1 (t4 @@' AE_FVar y)) (H & y ~ AC_Typ t1 & empty)).
+  repeat rewrite~ concat_empty_r.
+
+  apply aunify_middle_change in H4.
+  repeat rewrite concat_empty_r in *. auto.
+  rewrite~ concat_empty_r.
+
+  apply AUnify_Forall with (L \u dom G).
+  intros y notin.
+  assert(y \notin L) by auto.
+  assert(ok (G & y ~ AC_TVar)) by apply~ ok_push.
+  lets: H1 H2 H3. auto.
+
+  lets: atunify_ok_preservation uni1 okg.
+  apply* AUnify_Ann.
+Qed.
+
+Lemma resolve_evar_middle_change2: forall G1 G2 a t H1 H2 t2 v a0,
+    AResolveEVar (G1 & a ~ AC_Var & G2) a0 v t2
+                 (H1 & a ~ AC_Var & H2) ->
+    ok (G1 & a ~ AC_Var & G2) ->
+    AResolveEVar (G1 & a ~ AC_Typ t & G2) a0 v t2
+                 (H1 & a ~ AC_Typ t & H2).
+Proof.
+  introv res okg.
+  gen_eq S1: (G1 & a ~ AC_Var & G2).
+  gen_eq S2: (H1 & a ~ AC_Var & H2). gen H1 H2 G1 G2.
+  lets: resolve_evar_ok_preservation res okg.
+  induction res; introv sinfo1 sinfo2; subst; auto;
+    try(solve[apply ok_middle_eq2 in sinfo2; auto;
+              try(destruct sinfo2 as [? [_ ?]]; subst; constructor~);
+              try(rewrite~ <- sinfo2)]).
+
+  (* EVAR BEFORE *)
+  assert (binds a AC_Var (H1 & a ~ AC_Var & H2)).
+  apply binds_middle_eq. rewrite sinfo1 in okg. apply ok_middle_inv_r in okg. auto.
+  assert (a <> b). introv neq. subst.
+  rewrite <- sinfo1 in H0. do 2 rewrite <- concat_assoc in H0.
+  false binds_middle_eq_inv H0.
+  repeat rewrite~ concat_assoc.
+  assert (a <> a0). introv neq. subst.
+  rewrite <- sinfo1 in H0.
+  false binds_middle_eq_inv H0; auto.
+
+  rewrite <- sinfo1 in H0.
+  apply binds_remove in H0; auto.
+  rewrite <- concat_assoc in H0.
+  apply binds_remove in H0; auto.
+  rewrite concat_assoc in H0.
+  apply binds_concat_inv in H0.
+  destruct H0 as [bdg3 | [noting3 bdg1g2]].
+  apply split_bind_context in bdg3.
+  destruct bdg3 as (I1 & I2 & g3info). subst.
+  repeat rewrite concat_assoc in sinfo2.
+  apply ok_middle_eq2 in sinfo2; auto.
+  destruct sinfo2 as [? [_ ?]]. subst.
+  repeat rewrite concat_assoc in sinfo1.
+  apply ok_middle_eq2 in sinfo1; auto.
+  destruct sinfo1 as [? [_ ?]]. subst.
+
+  assert(
+      AResolveEVar
+     (G1 & b ~ AC_Unsolved_EVar & G2 & a0 ~ AC_Unsolved_EVar & (I1 & a ~ AC_Typ t & H2))
+     a0 (AT_EVar b) (AT_EVar b)
+     (G1 & b ~ AC_Unsolved_EVar & G2 & a0 ~ AC_Unsolved_EVar & (I1 & a ~ AC_Typ t & H2))).
+  apply~ AResolveEVar_EVar_Before.
+  repeat rewrite concat_assoc in H0; auto.
+
+  repeat rewrite concat_assoc in H. auto.
+  rewrite <- sinfo1.
+  repeat rewrite concat_assoc in H. auto.
+  repeat rewrite concat_assoc in H. auto.
+  rewrite <- sinfo2.
+  repeat rewrite concat_assoc in H. auto.
+
+  apply binds_concat_inv in bdg1g2.
+  destruct bdg1g2 as [bdg2 | [noting2 bdg1]].
+  apply split_bind_context in bdg2.
+  destruct bdg2 as (I1 & I2 & g2info). subst.
+  repeat rewrite concat_assoc in sinfo2.
+  do 2 rewrite <- concat_assoc in sinfo2.
+  apply ok_middle_eq2 in sinfo2; auto.
+  destruct sinfo2 as [? [_ ?]]. subst.
+  repeat rewrite concat_assoc in sinfo1.
+  do 2 rewrite <- concat_assoc in sinfo1.
+  apply ok_middle_eq2 in sinfo1; auto.
+  destruct sinfo1 as [? [_ ?]]. subst.
+
+  assert(
+   AResolveEVar
+     (G1 & b ~ AC_Unsolved_EVar & (I1 & a ~ AC_Typ t & I2) & a0 ~ AC_Unsolved_EVar & G3)
+     a0 (AT_EVar b) (AT_EVar b)
+     (G1 & b ~ AC_Unsolved_EVar & (I1 & a ~ AC_Typ t& I2) & a0 ~ AC_Unsolved_EVar & G3)).
+  apply~ AResolveEVar_EVar_Before.
+  repeat rewrite concat_assoc in H0; auto.
+  repeat rewrite concat_assoc. auto.
+
+  repeat rewrite concat_assoc in *. auto.
+  rewrite <- sinfo1.
+  repeat rewrite concat_assoc in *. auto.
+  repeat rewrite concat_assoc in *. auto.
+  rewrite <- sinfo2.
+  repeat rewrite concat_assoc in *. auto.
+
+  apply split_bind_context in bdg1.
+  destruct bdg1 as (I1 & I2 & g2info). subst.
+  do 4 rewrite <- concat_assoc in sinfo2.
+  apply ok_middle_eq2 in sinfo2; auto.
+  destruct sinfo2 as [? [_ ?]]. subst.
+  do 4 rewrite <- concat_assoc in sinfo1.
+  apply ok_middle_eq2 in sinfo1; auto.
+  destruct sinfo1 as [? [_ ?]]. subst.
+
+  repeat rewrite concat_assoc in *.
+  apply~ AResolveEVar_EVar_Before.
+
+  repeat rewrite concat_assoc in *. auto.
+  rewrite <- sinfo1.
+  repeat rewrite concat_assoc in *. auto.
+  repeat rewrite concat_assoc in *. auto.
+  rewrite <- sinfo2.
+  repeat rewrite concat_assoc in *. auto.
+
+  (* EVAR AFTER *)
+  assert( ok (H1 & a ~ AC_Var & H2)). rewrite <- sinfo1.
+  do 3 rewrite <- concat_assoc.
+  apply ok_insert; auto.
+  repeat rewrite concat_assoc.
+  apply* ok_middle_change.
+
+  assert (binds a AC_Var (H1 & a ~ AC_Var & H2)).
+  apply binds_middle_eq. apply ok_middle_inv_r in H3. auto.
+  assert (a <> b). introv neq. subst.
+  rewrite <- sinfo1 in H4.
+  false binds_middle_eq_inv H4.
+  rewrite~ sinfo1.
+  assert (a <> a0). introv neq. subst.
+  rewrite <- sinfo1 in H4.
+  do 2 rewrite <- concat_assoc in H4.
+  false binds_middle_eq_inv H4; auto.
+  repeat rewrite~ concat_assoc.
+  assert (a <> a1). introv neq. subst.
+  rewrite <- sinfo1 in H4.
+  do 3 rewrite <- concat_assoc in H4.
+  false binds_middle_eq_inv H4; auto.
+  repeat rewrite~ concat_assoc.
+
+  rewrite <- sinfo1 in H4.
+  apply binds_remove in H4; auto.
+  rewrite <- concat_assoc in H4.
+  apply binds_remove in H4; auto.
+  apply binds_remove in H4; auto.
+  rewrite concat_assoc in H4.
+  apply binds_concat_inv in H4.
+  destruct H4 as [bdg3 | [noting3 bdg1g2]].
+  apply split_bind_context in bdg3.
+  destruct bdg3 as (I1 & I2 & g3info). subst.
+  repeat rewrite concat_assoc in sinfo2.
+  apply ok_middle_eq2 in sinfo2; auto.
+  destruct sinfo2 as [? [_ ?]]. subst.
+  repeat rewrite concat_assoc in sinfo1.
+  apply ok_middle_eq2 in sinfo1; auto.
+  destruct sinfo1 as [? [_ ?]]. subst.
+
+  assert(
+   AResolveEVar
+     (G1 & a0 ~ AC_Unsolved_EVar & G2 & b ~ AC_Unsolved_EVar & (I1 & a ~ AC_Typ t & H2))
+     a0 (AT_EVar b) (AT_EVar a1)
+     (G1 & a1 ~ AC_Unsolved_EVar & a0 ~ AC_Unsolved_EVar & G2 & b ~ AC_Solved_EVar (AT_EVar a1) & (I1 & a ~ AC_Typ t & H2))).
+  apply~ AResolveEVar_EVar_After.
+  repeat rewrite concat_assoc in H1; auto.
+
+  repeat rewrite concat_assoc in *. auto.
+  repeat rewrite concat_assoc in *. auto.
+  rewrite <- sinfo2.
+  repeat rewrite concat_assoc in *. auto.
+
+  apply binds_concat_inv in bdg1g2.
+  destruct bdg1g2 as [bdg2 | [noting2 bdg1]].
+  apply split_bind_context in bdg2.
+  destruct bdg2 as (I1 & I2 & g2info). subst.
+  repeat rewrite concat_assoc in sinfo2.
+  do 2 rewrite <- concat_assoc in sinfo2.
+  apply ok_middle_eq2 in sinfo2; auto.
+  destruct sinfo2 as [? [_ ?]]. subst.
+  repeat rewrite concat_assoc in sinfo1.
+  do 2 rewrite <- concat_assoc in sinfo1.
+  apply ok_middle_eq2 in sinfo1; auto.
+  destruct sinfo1 as [? [_ ?]]. subst.
+
+  repeat rewrite concat_assoc.
+  assert(
+   AResolveEVar
+     (G1 & a0 ~ AC_Unsolved_EVar & (I1 & a ~ AC_Typ t & I2) &
+      b ~ AC_Unsolved_EVar & G3) a0 (AT_EVar b) (AT_EVar a1)
+     (G1 & a1 ~ AC_Unsolved_EVar & a0 ~ AC_Unsolved_EVar & (I1 & a ~ AC_Typ t &
+      I2) & b ~ AC_Solved_EVar (AT_EVar a1) & G3)).
+  apply~ AResolveEVar_EVar_After.
+  repeat rewrite concat_assoc in *; auto.
+
+  repeat rewrite concat_assoc in *. auto.
+  repeat rewrite concat_assoc in *. auto.
+  rewrite <- sinfo2.
+  repeat rewrite concat_assoc in *. auto.
+
+  apply split_bind_context in bdg1.
+  destruct bdg1 as (I1 & I2 & g2info). subst.
+  do 4 rewrite <- concat_assoc in sinfo2.
+  apply ok_middle_eq2 in sinfo2; auto.
+  destruct sinfo2 as [? [_ ?]]. subst.
+  do 5 rewrite <- concat_assoc in sinfo1.
+  apply ok_middle_eq2 in sinfo1; auto.
+  destruct sinfo1 as [? [_ ?]]. subst.
+
+  repeat rewrite concat_assoc.
+  apply~ AResolveEVar_EVar_After.
+  repeat rewrite concat_assoc in *; auto.
+
+  repeat rewrite concat_assoc in *. auto.
+  rewrite <- sinfo2.
+  repeat rewrite concat_assoc in *. auto.
+
+
+  (* PI *)
+  lets: resolve_evar_wextctx res okg.
+  apply weak_extension_order_var in H0.
+  destruct H0 as (I1 & I2 & [hinfo _]).
+  subst.
+  lets: resolve_evar_ok_preservation res okg.
+  apply AResolveEVar_Pi with (L:=L \u dom (I1 & a ~ AC_Var & I2) \u dom (H4 & a ~ AC_Var & H5)) (H1:=(I1 & a ~ AC_Typ t & I2)).
+  forwards * : IHres. clear IHres.
+  intros y notin.
+  assert(y \notin L) by auto.
+  lets: H2 H1. clear H2.
+  assert(H4 & a ~ AC_Var & H5 & y ~ AC_Var = H4 & a ~ AC_Var & (H5 & y ~ AC_Var )) by repeat rewrite~ concat_assoc.
+  assert(I1 & a ~ AC_Var & I2 & y ~ AC_Var = I1 & a ~ AC_Var & (I2 & y ~ AC_Var)) by  repeat rewrite~ concat_assoc.
+  assert (ok (I1 & a ~ AC_Var & I2 & y ~ AC_Var)) by apply~ ok_push.
+  lets: H3 H1 H8 H2 H7. apply~ ok_push.
+  repeat rewrite concat_assoc in H9; auto.
+
+  rewrite tsubst_add_ctx in H9. rewrite tsubst_add_var in H9.
+  rewrite tsubst_add_ctx. rewrite tsubst_add_typvar. auto.
+
+  (* APP *)
+  lets: resolve_evar_wextctx res1 okg.
+  apply weak_extension_order_var in H0.
+  destruct H0 as (I1 & I2 & [hinfo _]). subst.
+  lets: resolve_evar_ok_preservation res1 okg.
+  lets: resolve_evar_ok_preservation res2 H0.
+  forwards * : IHres1. clear IHres1.
+  forwards * : IHres2. clear IHres2.
+  apply* AResolveEVar_App.
+
+  rewrite tsubst_add_ctx in H5. rewrite tsubst_add_var in H5.
+  rewrite tsubst_add_ctx. rewrite tsubst_add_typvar. auto.
+
+  (* LAM *)
+  apply AResolveEVar_Lam with (L \u dom (G1 & a ~ AC_Var & G2) \u dom (H3 & a ~ AC_Var & H4)).
+  intros y notin.
+  assert(y \notin L) by auto.
+  lets: H1 H0. clear H1.
+  assert(H3 & a ~ AC_Var & H4 & y ~ AC_Var = H3 & a ~ AC_Var & (H4 & y ~ AC_Var )) by repeat rewrite~ concat_assoc.
+  assert(G1 & a ~ AC_Var & G2 & y ~ AC_Var = G1 & a ~ AC_Var & (G2 & y ~ AC_Var)) by  repeat rewrite~ concat_assoc.
+  assert (ok (G1 & a ~ AC_Var & G2 & y ~ AC_Var)) by apply~ ok_push.
+  assert (ok (H3 & a ~ AC_Var & H4 & y ~ AC_Var)) by apply~ ok_push.
+  lets: H2 H0 H7 H8 H1 H6.
+  repeat rewrite concat_assoc in H9; auto.
+
+  (* ANN *)
+  lets: resolve_evar_wextctx res1 okg.
+  apply weak_extension_order_var in H0.
+  destruct H0 as (I1 & I2 & [hinfo _]). subst.
+  lets: resolve_evar_ok_preservation res1 okg.
+  lets: resolve_evar_ok_preservation res2 H0.
+  forwards * : IHres1. clear IHres1.
+  forwards * : IHres2. clear IHres2.
+  apply* AResolveEVar_Ann.
+
+  rewrite tsubst_add_ctx in H5. rewrite tsubst_add_var in H5.
+  rewrite tsubst_add_ctx. rewrite tsubst_add_typvar. auto.
+Qed.
+
+Lemma tunify_wextctx: forall G m s t H,
+    ATUnify m G s t H ->
+    ok G ->
+    WExtCtx G H.
+Proof.
+  introv uni okg.
+  lets: atunify_ok_preservation uni okg.
+  induction uni; auto.
+
+  (* APP *)
+  lets: atunify_ok_preservation uni1 okg.
+  lets: IHuni1 okg H2.
+  lets: IHuni2 H2 H0.
+  lets: weak_extension_transitivity H3 H4. auto.
+
+  (* LAM *)
+  pick_fresh y.
+  assert (y \notin L) by auto.
+  assert(ok (G & y ~ AC_Var)). constructor~.
+  assert(ok (H & y ~ AC_Var)). constructor~.
+  lets: H2 y H3 H4 H5.
+  lets: weak_extension_remove_var H6.  auto.
+
+  (* PI *)
+  pick_fresh y.
+  assert (y \notin L) by auto.
+  assert(ok (G & y ~ AC_Typ t1)). constructor~.
+  lets: atunify_ok_preservation uni okg.
+  assert(ok (H1 & y ~ AC_Typ t1)). constructor~.
+  assert(ok (H & y ~ AC_Typ t1)). constructor~.
+  lets: H3 y H4 H7 H8.
+  lets: weak_extension_remove_typvar H9.
+  lets: IHuni okg H6.
+  lets: weak_extension_transitivity H11 H10. auto.
+
+  (* FORALL *)
+  pick_fresh y.
+  assert (y \notin L) by auto.
+  assert(ok (G & y ~ AC_TVar)). constructor~.
+  assert(ok (H & y ~ AC_TVar)). constructor~.
+  lets: H2 H3 H4 H5.
+  lets: weak_extension_remove_tvar H6.  auto.
+
+  (* ANN *)
+  lets: atunify_ok_preservation uni1 okg.
+  lets: IHuni1 okg H2.
+  lets: atunify_ok_preservation uni2 H2.
+  lets: IHuni2 H2 H4.
+  lets: weak_extension_transitivity H3 H5. auto.
+
+  (* EVarL *)
+  lets: resolve_evar_wextctx H3 okg. auto.
+  lets: weak_extension_solve_middle t2 H5. auto.
+
+  (* EVarR *)
+  lets: resolve_evar_wextctx H4 okg. auto.
+  lets: weak_extension_solve_middle t2 H6. auto.
+Qed.
+
+Lemma tunify_middle_change: forall e G1 G2 a m t d H1 H2,
+    ATUnify m (G1 & a ~ AC_Var & G2) e d (H1 & a ~ AC_Var & H2) ->
+    ok (G1 & a ~ AC_Var & G2) ->
+    ATUnify m (G1 & a ~ AC_Typ t & G2) e d (H1 & a ~ AC_Typ t & H2).
+Proof.
+  introv uni.
+  gen_eq S1: (G1 & a ~ AC_Var & G2).
+  gen_eq S2: (H1 & a ~ AC_Var & H2). gen H1 H2 G1 G2.
+  induction uni; introv sinfo1 sinfo2 okg; subst.
+
+  (* Var *)
+  apply ok_middle_eq2 in sinfo2; auto.
+  destruct sinfo2 as [? [_ ?]]. subst.
+  destruct(eq_var_dec x a).
+  subst.
+  apply~ ATUnify_Typed_Var. apply~ binds_middle_eq.
+  apply ok_middle_inv_r in okg. auto.
+  apply ATUnify_Var.
+  apply binds_remove in H; auto.
+  apply~ binds_weaken.
+  apply* ok_middle_change.
+  rewrite <- sinfo2. auto.
+
+  (* TypedVar *)
+  assert (x <> a). introv neq. subst. false binds_middle_eq_inv H. auto.
+  apply binds_remove in H; auto.
+  apply ok_middle_eq2 in sinfo2; auto.
+  destruct sinfo2 as [? [_ ?]]. subst.
+  apply ATUnify_Typed_Var with t0. apply~ binds_weaken.
+  apply* ok_middle_change.
+  rewrite <- sinfo2. auto.
+
+  (* EVar *)
+  assert (a0 <> a). introv neq. subst. false binds_middle_eq_inv H. auto.
+  apply binds_remove in H; auto.
+  apply ok_middle_eq2 in sinfo2; auto.
+  destruct sinfo2 as [? [_ ?]]. subst.
+  apply ATUnify_EVar. apply~ binds_weaken.
+  apply* ok_middle_change.
+  rewrite <- sinfo2. auto.
+
+  (* TFVar *)
+  assert (a0 <> a). introv neq. subst. false binds_middle_eq_inv H. auto.
+  apply binds_remove in H; auto.
+  apply ok_middle_eq2 in sinfo2; auto.
+  destruct sinfo2 as [? [_ ?]]. subst.
+  apply ATUnify_TVar. apply~ binds_weaken.
+  apply* ok_middle_change.
+  rewrite <- sinfo2. auto.
+
+  (* STAR *)
+  apply ok_middle_eq2 in sinfo2; auto.
+  destruct sinfo2 as [? [_ ?]]. subst.
+  apply ATUnify_Star.
+  rewrite <- sinfo2. auto.
+
+  (* APP *)
+  lets: tunify_wextctx uni1 okg.
+  apply weak_extension_order_var in H.
+  destruct H as (I1 & I2 & [hinfo _]). subst.
+  lets: atunify_ok_preservation uni1 okg.
+  forwards * : IHuni1. clear IHuni1.
+  forwards * : IHuni2. clear IHuni2.
+  apply* ATUnify_App.
+  rewrite subst_add_ctx in H3.
+  rewrite subst_add_var in H3.
+  rewrite subst_add_ctx in H3.
+  rewrite subst_add_var in H3.
+  rewrite subst_add_ctx.
+  rewrite subst_add_typvar.
+  rewrite subst_add_ctx.
+  rewrite subst_add_typvar. auto.
+
+  (* LAM *)
+  apply ATUnify_Lam with (L \u dom (G1 & a ~ AC_Var & G2)).
+  intros y notin.
+  assert(H: y \notin L) by auto.
+  lets: H0 H. clear H0.
+  assert(H2 & a ~ AC_Var & H3 & y ~ AC_Var = H2 & a ~ AC_Var & (H3 & y ~ AC_Var )) by repeat rewrite~ concat_assoc.
+  assert(G1 & a ~ AC_Var & G2 & y ~ AC_Var = G1 & a ~ AC_Var & (G2 & y ~ AC_Var)) by  repeat rewrite~ concat_assoc.
+  assert (ok (G1 & a ~ AC_Var & G2 & y ~ AC_Var)) by apply~ ok_push.
+  lets: H1 H H0 H5 H6.
+  repeat rewrite concat_assoc in H7; auto.
+
+  (* CASTUP *)
+  forwards * : IHuni.
+  apply~ ATUnify_CastUp.
+
+  (* CASTDOWN *)
+  forwards * : IHuni.
+  apply~ ATUnify_CastDn.
+
+  (* PI *)
+  lets: tunify_wextctx uni okg.
+  apply weak_extension_order_var in H.
+  destruct H as (I1 & I2 & [hinfo _]). subst.
+  lets: atunify_ok_preservation uni okg.
+  apply ATUnify_Pi with (L:=L \u dom (I1 & a ~ AC_Var & I2)) (H1:=(I1 & a ~ AC_Typ t & I2)).
+  forwards * : IHuni.
+
+  intros y notin.
+  assert(y \notin L) by auto.
+
+  assert(H3 & a ~ AC_Var & H4 & y ~ AC_Typ t1 = H3 & a ~ AC_Var & (H4 & y ~ AC_Typ t1)) by repeat rewrite~ concat_assoc.
+  assert(I1 & a ~ AC_Var & I2 & y ~ AC_Typ t1 = I1 & a ~ AC_Var & (I2 & y ~ AC_Typ t1)) by repeat rewrite~ concat_assoc.
+  assert(ok (I1 & a ~ AC_Var & I2 & y ~ AC_Typ t1)) by apply~ ok_push.
+  lets: H2 H1 H5 H6 H7.
+
+  repeat rewrite~ concat_assoc in H8.
+
+  rewrite tsubst_add_ctx in H8. rewrite tsubst_add_var in H8.
+  rewrite tsubst_add_ctx in H8. rewrite tsubst_add_var in H8.
+  rewrite tsubst_add_ctx. rewrite tsubst_add_typvar.
+  rewrite tsubst_add_ctx. rewrite tsubst_add_typvar. auto.
+
+  (* FORALL *)
+  apply ATUnify_Forall with (L \u dom (G1 & a ~ AC_Var & G2)).
+  intros y notin.
+  assert(H: y \notin L) by auto.
+  lets: H0 H. clear H0.
+  assert(H2 & a ~ AC_Var & H3 & y ~ AC_TVar = H2 & a ~ AC_Var & (H3 & y ~ AC_TVar)) by repeat rewrite~ concat_assoc.
+  assert(G1 & a ~ AC_Var & G2 & y ~ AC_TVar = G1 & a ~ AC_Var &  (G2 & y ~ AC_TVar)) by repeat rewrite~ concat_assoc.
+  assert (ok (G1 & a ~ AC_Var & G2 & y ~ AC_TVar)) by apply~ ok_push.
+  lets: H1 H H0 H5 H6.
+  repeat rewrite concat_assoc in H7; auto.
+
+  (* ANN *)
+  lets: tunify_wextctx uni1 okg.
+  apply weak_extension_order_var in H.
+  destruct H as (I1 & I2 & [hinfo _]). subst.
+  lets: atunify_ok_preservation uni1 okg.
+  forwards * : IHuni1. clear IHuni1.
+  forwards * : IHuni2 H.
+  apply* ATUnify_Ann.
+  rewrite tsubst_add_ctx in H3. rewrite tsubst_add_var in H3.
+  rewrite tsubst_add_ctx in H3. rewrite tsubst_add_var in H3.
+  rewrite tsubst_add_ctx. rewrite tsubst_add_typvar.
+  rewrite tsubst_add_ctx. rewrite tsubst_add_typvar. auto.
+
+  (* EVAR TY *)
+  lets: resolve_evar_ok_preservation H0 okg.
+  assert(binds a0 (AC_Solved_EVar t2) (H1 & a0 ~ AC_Solved_EVar t2 & H2)).
+  apply~ binds_middle_eq. apply ok_middle_inv_r in H6; auto.
+  rewrite sinfo1 in H7.
+  apply binds_remove in H7; auto.
+  apply binds_concat_inv in H7.
+  destruct H7 as [bdh2 | [notinh2 bdh1]].
+  apply split_bind_context in bdh2.
+  destruct bdh2 as (I1 & I2 & g2info). subst.
+  repeat rewrite concat_assoc in *.
+  apply ok_middle_eq2 in sinfo1; auto.
+  destruct sinfo1 as [? [_ ?]]. subst.
+  apply~ ATUnify_EVarTy.
+  do 3 rewrite <- concat_assoc in H0.
+  rewrite concat_assoc in H0.
+  apply resolve_evar_middle_change2 with (t:=t) in H0; auto.
+  repeat rewrite concat_assoc in H0. auto.
+  apply* awtermt_replace2.
+  apply* ok_middle_change.
+  rewrite <- sinfo1. apply* ok_middle_change.
+
+  apply split_bind_context in bdh1.
+  destruct bdh1 as (I1 & I2 & g2info). subst.
+  do 3 rewrite <- concat_assoc in sinfo1.
+  rewrite concat_assoc in sinfo1.
+  apply ok_middle_eq2 in sinfo1; auto.
+  destruct sinfo1 as [? [_ ?]]. subst.
+  do 3 rewrite <- concat_assoc.
+  rewrite concat_assoc.
+  apply~ ATUnify_EVarTy.
+  repeat rewrite concat_assoc in H0.
+  apply resolve_evar_middle_change2 with (t:=t) in H0; auto.
+  repeat rewrite concat_assoc. auto.
+  apply* ok_middle_change.
+  rewrite <- sinfo1. apply* ok_middle_change.
+
+  assert(a0 <> a). introv neq. subst. false binds_middle_eq_inv H7.
+  rewrite~ <- sinfo1. apply* ok_middle_change.
+  auto.
+
+  (* TY EVAR *)
+  lets: resolve_evar_ok_preservation H3 okg.
+  assert(binds a0 (AC_Solved_EVar t2) (H1 & a0 ~ AC_Solved_EVar t2 & H2)).
+  apply~ binds_middle_eq. apply ok_middle_inv_r in H7; auto.
+  rewrite sinfo1 in H8.
+  apply binds_remove in H8; auto.
+  apply binds_concat_inv in H8.
+  destruct H8 as [bdh2 | [notinh2 bdh1]].
+  apply split_bind_context in bdh2.
+  destruct bdh2 as (I1 & I2 & g2info). subst.
+  repeat rewrite concat_assoc in *.
+  apply ok_middle_eq2 in sinfo1; auto.
+  destruct sinfo1 as [? [_ ?]]. subst.
+  apply~ ATUnify_TyEVar.
+  do 3 rewrite <- concat_assoc in H3.
+  rewrite concat_assoc in H3.
+  apply resolve_evar_middle_change2 with (t:=t) in H3; auto.
+  repeat rewrite concat_assoc in H3. auto.
+  apply* awtermt_replace2.
+  apply* ok_middle_change.
+  rewrite <- sinfo1. apply* ok_middle_change.
+
+  apply split_bind_context in bdh1.
+  destruct bdh1 as (I1 & I2 & g2info). subst.
+  do 3 rewrite <- concat_assoc in sinfo1.
+  rewrite concat_assoc in sinfo1.
+  apply ok_middle_eq2 in sinfo1; auto.
+  destruct sinfo1 as [? [_ ?]]. subst.
+  do 3 rewrite <- concat_assoc.
+  rewrite concat_assoc.
+  apply~ ATUnify_TyEVar.
+  repeat rewrite concat_assoc in H3.
+  apply resolve_evar_middle_change2 with (t:=t) in H3; auto.
+  repeat rewrite concat_assoc. auto.
+  apply* ok_middle_change.
+  rewrite <- sinfo1. apply* ok_middle_change.
+
+  assert(a0 <> a). introv neq. subst. false binds_middle_eq_inv H8.
+  rewrite~ <- sinfo1. apply* ok_middle_change.
+  auto.
+
+  apply ATUnify_Expr.
+  forwards * : IHuni okg.
+Qed.
+
+Lemma aunify_is_atunify: forall G s t H,
+    ok G ->
+    AUnify G s t H ->
+    ATUnify UType G s t H.
+Proof.
+  introv okg uni.
+  induction uni; auto.
+  apply ATUnify_Expr. apply~ ATUnify_Var.
+  apply ATUnify_Expr. apply ATUnify_Typed_Var with t; auto.
+  apply ATUnify_EVar; auto.
+  apply ATUnify_TVar; auto.
+  apply ATUnify_Expr. apply ATUnify_Star; auto.
+
+  lets: unify_ok_preservation uni1 okg.
+  lets: IHuni1 okg. inversion H2; subst.
+  lets: IHuni2 H0. inversion H3; subst.
+  apply ATUnify_Expr. apply* ATUnify_App.
+
+  apply ATUnify_Expr.
+  apply ATUnify_Lam with (L \u dom G).
+  intros y notin.
+  assert(y \notin L) by auto.
+  assert(ok (G & y ~ AC_Var)) by apply~ ok_push.
+  lets: H0 H2. clear H0.
+  lets: H1 H2 H3. clear H1. inversion H0; subst.
+  auto.
+
+  lets: IHuni okg.
+  inversion H0; subst.
+  apply ATUnify_Expr. apply ATUnify_CastUp; auto.
+
+  lets: IHuni okg.
+  inversion H0; subst.
+  apply ATUnify_Expr. apply ATUnify_CastDn; auto.
+
+  apply ATUnify_Expr.
+  apply ATUnify_Pi with (L:=L \u dom H1) (H1:=H1); auto.
+  intros y notin.
+  assert(y \notin L) by auto.
+  lets: IHuni okg.
+  lets: atunify_ok_preservation H4 okg.
+  assert(ok (H1 & y ~ AC_Var)) by apply~ ok_push.
+  lets: H2 H3 H6. clear H2.
+
+  assert( ATUnify UType (H1 & y ~ AC_Var & empty) (ACtxTSubst H1 (t2 @@' AE_FVar y))
+         (ACtxTSubst H1 (t4 @@' AE_FVar y)) (H & y ~ AC_Var & empty)).
+  repeat rewrite~ concat_empty_r.
+
+  apply tunify_middle_change with (t:=t1) in H2.
+  repeat rewrite concat_empty_r in *. auto.
+  rewrite~ concat_empty_r.
+
+  apply ATUnify_Expr.
+  apply ATUnify_Forall with (L \u dom G).
+  intros y notin.
+  assert(y \notin L) by auto.
+  assert(ok (G & y ~ AC_TVar)) by apply~ ok_push.
+  lets: H1 H2 H3. auto.
+
+  lets: unify_ok_preservation uni1 okg.
+  lets: IHuni1 okg. inversion H2; subst.
+  lets: IHuni2 H0.
+  apply ATUnify_Expr. apply* ATUnify_Ann.
+
+  apply~ ATUnify_EVarTy.
+  apply~ ATUnify_TyEVar.
+Qed.
